theories/Algorithmic/Typing/Definitions.v
@@ -1,0 +1,84 @@
+From McPTS Require Import PtsSignature.
+From McPTS.Algorithmic.Subtyping Require Export Definitions.
+From McPTS.Core Require Import Base.
+From McPTS.Core.Semantic Require Export NbE.
+From McPTS.Core.Syntactic Require Export SystemOpt.
+Import Syntax_Notations.
+
+
+Reserved Notation "⟪ pred_P ⟫ Γ '⊢a' M ⟹ A" (in custom judg at level 80, pred_P constr, Γ custom exp, M custom exp, A custom exp).
+Reserved Notation "⟪ pred_P ⟫ Γ '⊢a' M ⟸ A" (in custom judg at level 80, pred_P constr, Γ custom exp, M custom exp, A custom exp).
+
+Generalizable All Variables.
+
+(* Record ConvertibleSig (P : PtsSig) : Type := *)
+(*   mkConvertibleSig { *)
+(*       Convert : ctx P -> typ P -> typ P -> Prop; *)
+(*       CorrectConv : forall Γ A B, Convert Γ A B <-> {{ Γ ⊢ A ⊆ B }}; *)
+(*       DecidableConv : forall Γ A B, (Convert Γ A B) \/ ~(Convert Γ A B); *)
+(*     }. *)
+(* Arguments Convert {_}. *)
+(* Arguments CorrectConv {_}. *)
+(* Arguments DecidableConv {_}. *)
+
+Inductive alg_type_check {P} (pred_P : PredicativeSig P) : ctx P -> typ P -> exp P -> Prop :=             
+(** Conversion *)
+| atc_conv : `( {{ ⟪ pred_P ⟫ Γ ⊢a M ⟹ A }} ->
+                {{ Γ ⊢a A ⊆ B }} ->
+                {{ ⟪ pred_P ⟫ Γ ⊢a M ⟸ B }} )
+              
+where "⟪ pred_P ⟫ Γ '⊢a' M ⟸ A" := (alg_type_check pred_P Γ A M) (in custom judg) : type_scope
+
+with alg_type_infer {P} (pred_P : PredicativeSig P) : ctx P -> typ P -> exp P -> Prop :=
+(** Variables *)
+| ati_var : `( {{ #x : A @ s ∈ Γ }} ->
+               nbe_ty Γ A B ->
+               {{ ⟪ pred_P ⟫ Γ ⊢a #x ⟹ B }} )
+
+(** Sorts *)
+| ati_st : `( Ax_typ P s1 s2 ->
+              {{ ⟪ pred_P ⟫  Γ ⊢a Sort@s1 ⟹ Sort@s2 }} )
+             
+(** Functions *)
+| atc_pi : `( forall {r : Ru_pi P s1 s2 s3},
+                 {{ ⟪ pred_P ⟫  Γ ⊢a A ⟸ Sort@s1 }} ->
+                 {{ ⟪ pred_P ⟫  Γ, A@s1 ⊢a B ⟸ Sort@s2 }} ->
+                 {{ ⟪ pred_P ⟫  Γ ⊢a Π r A B ⟹ Sort@s3 }} )
+
+| ati_lam : `( forall {r : Ru_pi P s1 s2 s3},
+                  {{ ⟪ pred_P ⟫ Γ ⊢a A ⟸ Sort@s1 }} ->
+                  {{ ⟪ pred_P ⟫ Γ, A@s1 ⊢a B ⟸ Sort@s2 }} ->
+                  {{ ⟪ pred_P ⟫ Γ, A@s1 ⊢a M ⟹ B }} ->
+                  {{ ⟪ pred_P ⟫ Γ ⊢a λ r A M ⟹ Π r A B }} )
+             
+| ati_app : `( forall {r : Ru_pi P s1 s2 s3},
+                  {{ ⟪ pred_P ⟫ Γ ⊢a M ⟹ Π r A B }} ->
+                  {{ ⟪ pred_P ⟫ Γ ⊢a N ⟸ A }} ->
+                  {{ ⟪ pred_P ⟫ Γ ⊢a M N ⟹ B[Id,,N] }} )
+                  
+(** Naturals *)
+| ati_nat : `( Ru_nat P s ->
+               {{ ⟪ pred_P ⟫ Γ ⊢a ℕ ⟹ Sort@s }} )
+| ati_zero : `( Ru_nat P s ->
+                {{ ⟪ pred_P ⟫ Γ ⊢a zero ⟹ ℕ }} )
+| ati_succ : `( Ru_nat P s ->
+                {{ ⟪ pred_P ⟫ Γ ⊢a M ⟹ ℕ }} ->
+                {{ ⟪ pred_P ⟫ Γ ⊢a succ M ⟹ ℕ }} )
+| ati_rec : `( Ru_nat P s ->
+               {{ ⟪ pred_P ⟫ Γ, ℕ@s ⊢a A ⟸ Sort@s' }} ->
+               {{ ⟪ pred_P ⟫ Γ ⊢a MZ ⟸ A[Id,,zero] }} ->
+               {{ ⟪ pred_P ⟫ Γ, ℕ@s, A@s' ⊢a MS ⟸ A[Wk∘Wk,,succ #1] }} ->
+               {{ ⟪ pred_P ⟫ Γ ⊢a N ⟸ ℕ }} ->
+               nbe_ty Γ {{{ A[Id,,N] }}} B
+               {{ ⟪ pred_P ⟫ Γ ⊢a rec N return A | zero -> MZ | succ -> MS end ⟹ B }} )
+where "⟪ pred_P ⟫ Γ '⊢a' M ⟹ A" := (alg_type_infer pred_P Γ A M) (in custom judg) : type_scope.
+
+
+#[export]
+Hint Constructors alg_type_check alg_type_infer : mcpts.
+
+Scheme alg_type_check_mut_ind := Induction for alg_type_check Sort Prop
+with alg_type_infer_mut_ind := Induction for alg_type_infer Sort Prop.
+Combined Scheme alg_type_mut_ind from
+  alg_type_check_mut_ind,
+  alg_type_infer_mut_ind.
