theories/Algorithmic/Typing/Lemmas.v
@@ -1,0 +1,498 @@
+From McPTS Require Import PtsSignature LibTactics.
+From McPTS.Algorithmic Require Import Definitions.
+From McPTS.Core Require Import Base.
+(* From McPTS.Core.Completeness Require Import Consequences.Rules. *)
+(* From McPTS.Core.Semantic Require Import Consequences. *)
+From McPTS.Frontend Require Import Elaborator.
+Import Domain_Notations.
+
+Record FunctionalSig (P : PtsSig) : Prop :=
+  mkFunctionalSig {
+      Func_ax_typ : forall s1 s2 s2', Ax_typ P s1 s2 -> Ax_typ P s1 s2' -> s2 = s2';
+      Func_ru_pi : forall s1 s2 s3 s3', Ru_pi P s1 s2 s3 -> Ru_pi P s1 s2 s3' -> s3 = s3';
+      Func_ru_nat : forall s s', Ru_nat P s -> Ru_nat P s' -> s = s';
+    }.
+
+
+
+Lemma functional_alg_type_infer {P} (conv_P : ConvertibleSig P) (func_P : FunctionalSig P) : forall {Γ : ctx P} {A A' M},
+    {{ ⟪ conv_P ⟫ Γ ⊢a M ⟹ A }} ->
+    {{ ⟪ conv_P ⟫ Γ ⊢a M ⟹ A' }} ->
+    A = A'.
+Proof.
+  intros * HM1 HM2. gen A'.
+  induction HM1;
+    intros;
+    dependent destruction HM2;
+    subst;
+    functional_nbe_rewrite_clear;
+    f_equiv;
+    try reflexivity;
+    intuition.
+
+  - assert (A = A') as <- by (eapply functional_ctx_lookup; eassumption).
+    reflexivity.  
+  - assert ({{{ Π r A B }}} = {{{ Π r0 A0 B0 }}}) by mauto 2.
+    inversion_clear H1.
+    reflexivity.
+  - eapply Func_ru_nat; mauto 2.
+Qed.
+
+#[local]
+Hint Resolve functional_alg_type_infer : mcpts.
+
+Ltac functional_alg_type_infer_rewrite_clear1 :=
+  let tactic_error o1 o2 := fail 3 "functional_alg_type_infer equality between" o1 "and" o2 "cannot be solved by mauto" in
+  match goal with
+  | H1 : {{ ⟪ ?conv_P ⟫ ^?Γ ⊢a ^?M ⟹ ^?A1 }}, H2 : {{ ⟪ ?conv_P ⟫ ^?Γ ⊢a ^?M ⟹ ^?A2 }} |- _ =>
+      clean replace A2 with A1 by first [solve [mauto 2 using functional_alg_type_infer] | tactic_error A2 A1]; clear H2
+  end.
+Ltac functional_alg_type_infer_rewrite_clear := repeat functional_alg_type_infer_rewrite_clear1.
+
+    
+Lemma alg_type_sound {P} (conv_P : ConvertibleSig P) :
+  (forall {Γ : ctx P} {A M}, {{ ⟪ conv_P ⟫ Γ ⊢a M ⟸ A }} -> {{ ⊢ Γ }} -> {{ Γ ⊢ A }} -> {{ Γ ⊢ M : A }}) /\
+    (forall {Γ : ctx P} {A M}, {{ ⟪ conv_P ⟫ Γ ⊢a M ⟹ A }} -> {{ ⊢ Γ }} -> {{ Γ ⊢ M : A }}).
+Proof.
+  apply alg_type_mut_ind; intros; try mautosolve 4.
+
+  - assert {{ Γ ⊢ M : A }} by mauto 2.
+    assert {{ Γ ⊢ A ⊆ B }} by (eapply CorrectConv; mauto 2).
+    mauto 2.
+    
+  - assert {{ Γ ⊢ A : Sort@s1 }} by mauto 3.
+    assert {{ ⊢ Γ, A@s1 }} by mauto 3.
+    assert {{ Γ, A@s1 ⊢ B : Sort@s2 }} by mauto 3.
+    mauto 3.
+
+  - assert {{ Γ ⊢ A : Sort@s1 }} by mauto 3.
+    assert {{ ⊢ Γ, A@s1 }} by mauto 3.
+    assert {{ Γ, A@s1 ⊢ B : Sort@s2 }} by mauto 3.
+    assert {{ Γ, A@s1 ⊢ M : B }} by mauto 3.
+    mauto 3.
+
+  - assert {{ Γ ⊢ M : Π r A B }} by mauto 2.
+    gen_presup H2.
+    eapply wf_typ_pi_inversion in HAwf as [].
+    assert {{ Γ ⊢ N : A }} by mauto 3.
+    mauto 2.
+    
+  - assert {{ Γ ⊢ ℕ : Sort@s }} by mauto 2.
+    assert {{ ⊢ Γ, ℕ@s }} by mauto 2.
+    assert {{ Γ, ℕ@s ⊢ A : Sort@s' }} by mauto 3.
+    assert {{ ⊢ Γ, ℕ@s, A@s' }} by mauto 3.
+    assert {{ Γ ⊢ N : ℕ }} by mauto 2.
+    assert {{ Γ ⊢s Id,,zero : Γ, ℕ@s }} by mauto 3.
+    assert {{ Γ ⊢ A[Id,,zero] : Sort@s' }} by mauto 3.
+    assert {{ Γ, ℕ@s, A@s' ⊢s Wk∘Wk : Γ }} by (econstructor; mauto 3).
+    assert {{ Γ, ℕ@s, A@s' ⊢s Wk∘Wk,,succ #1 : Γ, ℕ@s }} by mauto 4.
+    assert {{ Γ, ℕ@s, A@s' ⊢ A[Wk∘Wk,,succ #1] : Sort@s' }} by mauto 4.
+    simpl.
+    econstructor; mauto 3.
+Qed.
+
+
+Lemma alg_type_check_sound {P} (conv_P : ConvertibleSig P) : forall {Γ : ctx P} {A M},
+    {{ ⟪ conv_P ⟫ Γ ⊢a M ⟸ A }} ->
+    {{ ⊢ Γ }} ->
+    {{ Γ ⊢ A }} ->
+    {{ Γ ⊢ M : A }}.
+Proof.
+  pose proof (alg_type_sound conv_P); intuition.
+Qed.
+
+Lemma alg_type_infer_sound {P} (conv_P : ConvertibleSig P) : forall {Γ : ctx P} {A M},
+    {{ ⟪ conv_P ⟫ Γ ⊢a M ⟹ A }} -> {{ ⊢ Γ }} -> {{ Γ ⊢ M : A }}.
+Proof.
+  pose proof @alg_type_sound; intuition.
+Qed.
+
+
+(* Lemma alg_type_infer_normal {P} (conv_P : ConvertibleSig P) : forall {Γ : ctx P} {A A' M}, *)
+(*     {{ ⊢ Γ }} -> *)
+(*     {{ Γ ⊢a M ⟹ A }} -> *)
+(*     nbe_ty Γ A A' -> *)
+(*     A = A'. *)
+(* Proof with (f_equiv; mautosolve 4). *)
+(*   intros. *)
+(*   eapply idempotent_nbe_ty; mauto 2. *)
+  
+  
+(*   intros * ? Hinfer Hnbe. gen A'. *)
+(*   assert {{ Γ ⊢ M : A }} by mauto 3 using alg_type_infer_sound. *)
+(*   induction Hinfer; intros; *)
+(*     try (dir_inversion_clear_by_head nbe_ty; *)
+(*          dir_inversion_by_head eval_exp; subst; *)
+(*          dir_inversion_by_head read_typ; subst; *)
+(*          reflexivity). *)
+(*   - assert {{ Γ ⊢ ℕ : Type@0 }} by mauto 3. *)
+(*     assert {{ Γ ⊢ M : ℕ }} by mauto 3 using alg_type_check_sound. *)
+(*     assert {{ ⊢ Γ, ℕ }} by mauto 3. *)
+(*     assert {{ Γ, ℕ ⊢ A : ^n{{{ Type@i }}} }} by mauto 3 using alg_type_infer_sound... *)
+(*   - assert {{ Γ ⊢ A : ^n{{{ Type@i }}} }} by mauto 3 using alg_type_infer_sound. *)
+(*     assert {{ Γ ⊢ A ≈ C : Type@i }} by mauto 3 using soundness_ty'. *)
+(*     assert {{ Γ, A ⊢ M : B }} by mauto 3 using alg_type_infer_sound. *)
+(*     assert (exists j, {{ Γ, A ⊢ B : Type@j }}) as [j] by (gen_presups; eauto 2). *)
+(*     assert {{ ⊢ Γ, A ≈ Γ, ^(C : exp) }} by mauto 3. *)
+(*     dir_inversion_clear_by_head nbe_ty. *)
+(*     simplify_evals. *)
+(*     dir_inversion_by_head read_typ; subst. *)
+(*     functional_initial_env_rewrite_clear. *)
+(*     assert (initial_env {{{ Γ, ^(C : exp) }}} d{{{ ρ ↦ ⇑! a (length Γ) }}}) by mauto 3. *)
+(*     assert (nbe_ty Γ A C) by mauto 3. *)
+(*     assert (nbe_ty Γ C A0) by mauto 3. *)
+(*     replace A0 with C by mauto 2. *)
+(*     assert (nbe_ty {{{ Γ, ^(C : exp) }}} B B') by mauto 3. *)
+(*     assert (nbe_ty {{{ Γ, A }}} B B') by mauto 4 using ctxeq_nbe_ty_eq'... *)
+(*   - assert {{ Γ ⊢ M : ^n{{{ Π A B }}} }} by mauto 3 using alg_type_infer_sound. *)
+(*     assert (exists i, {{ Γ ⊢ Π A B : Type@i }}) as [i] by (gen_presups; eauto 2). *)
+(*     assert ({{ Γ ⊢ A : Type@i }} /\ {{ Γ, ^(A : exp) ⊢ B : Type@i }}) as [] by mauto 3. *)
+(*     assert {{ Γ ⊢ N : A }} by mauto 3 using alg_type_check_sound. *)
+(*     assert {{ Γ ⊢ B[Id,,N] : Type@i }} by mauto 3... *)
+(*   - assert {{ Γ ⊢ A : Type@i }} by (eapply alg_type_sound in Hinfer1; mauto 3). *)
+(*     assert {{ Γ , A ⊢ B : Type@j }} by (eapply alg_type_sound in Hinfer2; mauto 3). *)
+(*     assert (exists j, {{ Γ ⊢ Σ A' C : Type@j }}) as [k] by (gen_presups; eauto 2). *)
+(*     apply wf_sigma_inversion' in H7; fold nf_to_exp in *. destruct_all. *)
+(*     dir_inversion_clear_by_head nbe_ty. *)
+(*     simplify_evals. *)
+(*     dir_inversion_by_head read_typ; subst. *)
+(*     assert (nbe_ty Γ A A' ) by mauto 3. *)
+(*     assert (nbe_ty Γ A' A0 ) by mauto 3. *)
+(*     replace A0 with A' in * by mauto 3. *)
+(*     assert {{ Γ ⊢ A ≈ A' : Type@i }} by mauto 3 using soundness_ty'. *)
+(*     functional_initial_env_rewrite_clear. *)
+(*     simplify_evals. *)
+(*     assert (nbe_ty {{{ Γ, A }}} B C) by unshelve mauto 3. *)
+(*     assert (nbe_ty {{{ Γ,  ^(A' : exp)}}} C B') by mauto 4. *)
+(*     assert {{ ⊢ Γ, A ≈ Γ, ^(A' : exp) }} by mauto 3. *)
+(*     assert (nbe_ty {{{ Γ, ^(A : exp) }}} C B') by mauto 3 using ctxeq_nbe_ty_eq'. *)
+(*     replace B' with C in * by mauto 3... *)
+(*   - assert {{ Γ ⊢ M : ^n{{{ Σ A B }}} }} by mauto 3 using alg_type_infer_sound. *)
+(*     gen_presups. *)
+(*     assert (nbe_ty Γ {{{Σ A B }}} n{{{Σ A B}}}). { *)
+(*       assert {{ Γ ⊢ ^ n{{{ Σ A B }}} ≈ ^ n{{{ Σ A B }}} : Type@i }} by (eapply exp_eq_refl; mauto 3). *)
+(*       apply completeness_ty in H as IH. destruct_all. *)
+(*       eapply IHHinfer in H2; subst; auto. *)
+(*     } *)
+(*     dir_inversion_clear_by_head nbe. *)
+(*     dir_inversion_clear_by_head nbe_ty. *)
+(*     simplify_evals. *)
+(*     dir_inversion_by_head read_typ; subst. *)
+(*     functional_initial_env_rewrite_clear. *)
+(*     simplify_evals. *)
+(*     functional_read_rewrite_clear. reflexivity. *)
+(*   - assert {{ Γ ⊢ M : ^n{{{ Σ A B }}} }} by mauto 3 using alg_type_infer_sound. *)
+(*     gen_presups. *)
+(*     apply wf_sigma_inversion' in HA; fold nf_to_exp in *. *)
+(*     destruct_all. *)
+(*     assert {{ Γ ⊢ fst M : A }} by mauto 3. *)
+(*     assert {{ Γ ⊢ B[Id,,fst M] : Type@i }} by mauto 3. *)
+(*     mauto 3. *)
+(*   - assert {{ Γ ⊢ A : ^n{{{ Type@i }}} }} by mauto 3 using alg_type_infer_sound. *)
+(*     assert {{ Γ ⊢ M : A }} by mauto 3 using alg_type_check_sound. *)
+(*     dir_inversion_clear_by_head nbe. *)
+(*     dir_inversion_clear_by_head nbe_ty. *)
+(*     simplify_evals. *)
+(*     dir_inversion_by_head read_typ; subst. *)
+(*     functional_initial_env_rewrite_clear. *)
+(*     functional_read_rewrite_clear. *)
+(*     assert (nbe_ty Γ A C) by mauto 3. *)
+(*     assert (nbe_ty Γ C A0) by mauto 3. *)
+(*     replace A0 with C in * by mauto 3. *)
+(*     assert (nbe Γ M A N) by mauto 3. *)
+(*     assert {{ Γ ⊢ A ≈ C : Type@i }} by mauto 2 using soundness_ty'. *)
+(*     assert (nbe Γ N C M1) by mauto 2. *)
+(*     replace M1 with N in * by mauto 2. *)
+(*     reflexivity. *)
+(*   - assert {{ Γ ⊢ A : ^n{{{ Type@i }}} }} by mauto 3 using alg_type_infer_sound. *)
+(*     assert {{ Γ ⊢ M1 : A }} by mauto 3 using alg_type_check_sound. *)
+(*     assert {{ Γ ⊢ M2 : A }} by mauto 3 using alg_type_check_sound. *)
+(*     assert {{ Γ ⊢ N : Eq A M1 M2 }} by mauto 3 using alg_type_check_sound. *)
+(*     assert {{ Γ, A ⊢s Wk : Γ }} by mauto 3. *)
+(*     assert {{ Γ, A ⊢ A[Wk] : Type@i }} by mauto 3. *)
+(*     assert {{ ⊢ Γ, A, A[Wk] }} by mauto 3. *)
+(*     assert {{ Γ, A, A[Wk] ⊢ Eq A[Wk∘Wk] #1 #0 : Type@i }} by mauto 3. *)
+(*     assert {{ Γ, A, A[Wk], Eq A[Wk∘Wk] #1 #0 ⊢ B : ^n{{{ Type@j }}} }} by mauto 3 using alg_type_infer_sound. *)
+(*     assert {{ Γ ⊢s Id,,M1,,M2,,N : Γ, A, A[Wk], Eq A[Wk∘Wk] #1 #0 }} by mauto 2. *)
+(*     assert {{ Γ ⊢ B[Id,,M1,,M2,,N] : Type@j }} by mauto 2. *)
+(*     mauto 3. *)
+(*   - assert (exists i, {{ Γ ⊢ A : Type@i }}) as [i] by mauto 2... *)
+(* Qed. *)
+
+(* #[export] *)
+(* Hint Resolve alg_type_infer_normal : mcpts. *)
+
+
+Lemma subtyp_sort_is_sort_helper {P} : forall {Γ : ctx P} {A B},
+    {{ Γ ⊢ A ⊆ B }} ->
+    forall s, {{ Γ ⊢ B ≈ Sort@s }} ->
+    exists s', {{ Γ ⊢ A ≈ Sort@s' }} /\ st_subtyp s' s.
+Proof.
+  intros * Hsub.
+  induction Hsub; intros.
+  - eexists; split; mauto 2.
+  - specialize (IHHsub2 s ltac:(eassumption)) as [s' []].
+    specialize (IHHsub1 s' ltac:(eassumption)) as [s'' []].
+    eexists; split; mauto 3.
+    etransitivity; eassumption.
+  - (* This is part of Completeness.Consequences.Types, not yet merged *)
+    assert (s2 = s) by admit. (* (eapply typ_eq_sort_implies_eq_level; mauto 2) *)
+    subst.
+    exists s1; split; mauto 3.
+  - (* This also need the consequences *)
+    assert ({{{ Π r A' B' }}} = {{{ Sort@s }}}) by admit.
+    inversion H5.
+Admitted.
+
+Lemma subtyp_sort_is_sort {P} : forall {Γ : ctx P} {A s},
+    {{ Γ ⊢ A ⊆ Sort@s }} ->
+    exists s', {{ Γ ⊢ A ≈ Sort@s' }} /\ st_subtyp s' s.
+Proof.
+  intros.
+  gen_presup H.
+  eapply subtyp_sort_is_sort_helper; mauto 2.
+Qed.
+
+  
+Lemma alg_type_check_typ_implies_alg_type_infer_typ {P} (conv_P : ConvertibleSig P) : forall {Γ A s},
+    {{ ⊢ Γ }} ->
+    {{ ⟪ conv_P ⟫ Γ ⊢a A ⟸ Sort@s }} ->
+    exists A' s', {{ ⟪ conv_P ⟫ Γ ⊢a A ⟹ A' }} /\ {{ Γ ⊢ A' ≈ Sort@s' }} /\ st_subtyp s' s.
+Proof.
+  intros * ? Hcheck.
+  inversion Hcheck as [? A' ? ? Hinfer Hsub]; subst.
+  assert {{ Γ ⊢ A' ⊆ Sort@s }} by (eapply CorrectConv; mauto 2).
+  pose proof (subtyp_sort_is_sort H0) as [s' []].
+  repeat eexists; mauto 3.
+Qed.
+
+#[export]
+Hint Resolve alg_type_check_typ_implies_alg_type_infer_typ : mcpts.
+
+Lemma alg_type_check_pi_implies_alg_type_infer_pi {P} (conv_P : ConvertibleSig P) : forall {Γ M A B s1 s2 s3 s} {r : Ru_pi P s1 s2 s3},
+    {{ ⊢ Γ }} ->
+    {{ Γ ⊢ Π r A B : Sort@s }} ->
+    {{ ⟪ conv_P ⟫ Γ ⊢a M ⟸ Π r A B }} ->
+    exists A' A0 B0, {{ ⟪ conv_P ⟫ Γ ⊢a M ⟹ A' }} /\ {{ Γ ⊢ A' ≈ Π r A0 B0 }} /\ {{ Γ ⊢ A0 ≈ A : Sort@s1 }} /\ (Convert conv_P {{{ Γ, A@s1 }}} B0 B).
+Proof.
+  intros * ? ? Hcheck.
+  assert ({{ Γ ⊢ A : Sort@s1 }} /\ {{ Γ, A@s1 ⊢ B : Sort@s2 }} /\ {{ Γ ⊢ Sort@s3 ⊆ Sort@s }}) as [? []] by mauto 3.
+  inversion Hcheck as [? A' ? ? Hinfer Hsub]; subst.
+  assert {{ Γ ⊢ A' ⊆ Π r A B }} by (eapply CorrectConv; mauto 3).
+  (* This should follow by consequences of normalization *)
+  assert (exists A0 B0, {{ Γ ⊢ A' ≈ Π r A0 B0 }} /\ {{ Γ ⊢ A0 ≈ A : Sort@s1 }} /\ {{ Γ, A0@s1 ⊢ B0 ⊆ B }}) as [A0 [B0 [? []]]] by admit.
+  repeat eexists; mauto 3.
+  assert {{ ⊢ Γ, A0@s1 ≈ Γ, A@s1 }} by mauto 3.
+  assert {{ Γ, A@s1 ⊢ B0 ⊆ B }} by mauto 3.
+  eapply CorrectConv; mauto 3.
+Admitted.
+
+
+#[export]
+Hint Resolve alg_type_check_pi_implies_alg_type_infer_pi : mcpts.
+
+Lemma alg_type_check_subtyp {P} (conv_P : ConvertibleSig P) : forall {Γ A A' M},
+    {{ ⟪ conv_P ⟫ Γ ⊢a M ⟸ A }} ->
+    {{ Γ ⊢ A ⊆ A' }} ->
+    {{ ⟪ conv_P ⟫ Γ ⊢a M ⟸ A' }}.
+Proof.
+  intros * [] **.
+  assert {{ Γ0 ⊢ A0 ⊆ B }} by (eapply CorrectConv; mauto 2).
+  assert {{ Γ0 ⊢ A0 ⊆ A' }} by mauto 2.
+  assert (Convert conv_P Γ0 A0 A') by (eapply CorrectConv; mauto 2).
+  mauto 2.
+Qed.
+
+#[export]
+Hint Resolve alg_type_check_subtyp : mcpts.
+
+Corollary alg_type_check_conv {P} (conv_P : ConvertibleSig P) : forall {Γ A A' M},
+    {{ ⟪ conv_P ⟫ Γ ⊢a M ⟸ A }} ->
+    {{ Γ ⊢ A ≈ A' }} ->
+    {{ ⟪ conv_P ⟫ Γ ⊢a M ⟸ A' }}.
+Proof.
+  mauto 3.
+Qed.
+
+#[export]
+Hint Resolve alg_type_check_conv : mcpts.
+
+Lemma alg_type_check_complete {P} (conv_P : ConvertibleSig P) : forall {Γ A M},
+    user_exp P M ->
+    {{ Γ ⊢ M : A }} ->
+    {{ ⟪ conv_P ⟫ Γ ⊢a M ⟸ A }}.
+Proof.
+  intros * Hue.
+  induction 1; gen_presups; inversion Hue; subst; clear Hue; mauto 4 using alg_type_check_subtyp.
+  - econstructor; mauto 3.
+    eapply CorrectConv; mauto 2.
+
+  - assert (Convert conv_P Γ {{{ Sort@s3 }}} {{{ Sort@s3 }}}) by (eapply CorrectConv; mauto 3).
+    econstructor; mauto 3.
+    econstructor; mauto 3.
+
+  - assert {{ ⟪ conv_P ⟫ Γ ⊢a A ⟸ Sort@s1 }} by mauto 2.
+    assert {{ ⟪ conv_P ⟫ Γ, A@s1 ⊢a M ⟸ B }} by mauto 2.
+    inversion_clear H3.
+    assert {{ Γ, A@s1 ⊢ A0 ⊆ B }} by (eapply CorrectConv; mauto 3).
+    assert {{ Γ ⊢ Π r A A0 ⊆ Π r A B }} by admit.
+    assert (Convert conv_P Γ {{{ Π r A A0 }}} {{{ Π r A B }}}) by (eapply CorrectConv; mauto 3).
+    econstructor; mauto 3.
+    econstructor; mauto 3.
+    admit.
+
+
+  - assert {{ ⟪ conv_P ⟫ Γ ⊢a M ⟸ Π r A B }} by mauto 2.
+    assert {{ ⟪ conv_P ⟫ Γ ⊢a N ⟸ A }} by mauto 2.
+    econstructor; mauto 3.
+    
+    
+  - econstructor; mauto 3.
+    mauto using alg_subtyping_complete.
+  - assert (exists j, {{ Γ, ℕ ⊢a A ⟹ Type@j }} /\ j <= i) as [j []] by mauto 3.
+    assert {{ Γ ⊢ A[Id,,M] : Type@i }} by mauto 3.
+    assert {{ Γ ⊢ A[Id,,M] ≈ A[Id,,M] : Type@i }} as [? [? _]]%completeness_ty by mauto 3.
+    econstructor; mauto using alg_subtyping_complete, soundness_ty'.
+  - assert (exists j, {{ Γ ⊢a A ⟹ Type@j }} /\ j <= i) as [j []] by mauto 3.
+    assert {{ ⊢ Γ, A }} by mauto 3.
+    assert (exists j, {{ Γ, A ⊢a B ⟹ Type@j }} /\ j <= i) as [j' []] by mauto 3.
+    assert (max j j' <= i) by lia.
+    econstructor; mauto 3 using alg_subtyping_complete.
+  - assert (exists j, {{ Γ ⊢a A ⟹ Type@j }} /\ j <= i) as [j []] by mauto 3.
+    assert {{ Γ, A ⊢a M ⟸ B }} by mauto 3.
+    assert (exists B', {{ Γ, A ⊢a M ⟹ B' }} /\ {{ Γ, A ⊢a B' ⊆ B }}) as [B' []] by (inversion_clear_by_head alg_type_check; firstorder).
+    assert (exists W, nbe_ty Γ A W /\ {{ Γ ⊢ A ≈ W : Type@i }}) as [W []] by mauto 3 using soundness_ty.
+    assert {{ ⊢ Γ, A }} by mauto 3.
+    assert {{ Γ, A ⊢ M : B' }} by mauto 3 using alg_type_infer_sound.
+    assert (exists j, {{ Γ, A ⊢ B' : Type@j }}) as [] by (gen_presups; eauto 2).
+    econstructor; mauto 3.
+    eapply alg_subtyping_complete.
+    eapply wf_subtyp_pi'; mauto 2.
+    mauto 4 using alg_subtyping_sound, lift_exp_max_left, lift_exp_max_right.
+  - assert {{ Γ ⊢a M ⟸ Π A B }} by mauto 2.
+    assert {{ Γ ⊢a N ⟸ A }} by mauto 2.
+    assert (exists A' B', {{ Γ ⊢a M ⟹ Π A' B' }} /\ {{ Γ ⊢ A' ≈ A : Type@i }} /\ {{ Γ, A ⊢a B' ⊆ B }}) as [A' [B' [? []]]] by mauto 3.
+    assert {{ Γ ⊢ M : ^n{{{ Π A' B' }}} }} by mauto 3 using alg_type_infer_sound.
+    assert (exists j, {{ Γ ⊢ Π A' B' : Type@j }}) as [j] by (gen_presups; eauto 2).
+    assert ({{ Γ ⊢ A' : Type@j }} /\ {{ Γ, ^(A' : exp) ⊢ B' : Type@j }}) as [] by mauto 3.
+    assert {{ Γ ⊢ N : A' }} by mauto 3.
+    assert {{ Γ ⊢ B'[Id,,N] : Type@j }} by mauto 3.
+    assert (exists W, nbe_ty Γ {{{ B'[Id,,N] }}} W /\ {{ Γ ⊢ B'[Id,,N] ≈ W : Type@j }}) as [W []] by (eapply soundness_ty; mauto 3).
+    assert {{ Γ, A ⊢ B' : Type@j }} by mauto 4.
+    assert {{ Γ, A ⊢ B' ⊆ B }} by mauto 4 using alg_subtyping_sound, lift_exp_max_left, lift_exp_max_right.
+    assert {{ Γ ⊢ B'[Id,,N] ⊆ B[Id,,N] }} by mauto 3.
+    assert {{ Γ ⊢ W ⊆ B[Id,,N] }} by (transitivity {{{ B'[Id,,N] }}}; mauto 3).
+    econstructor; mauto 4 using alg_subtyping_complete.
+  - assert (exists j, {{ Γ ⊢a A ⟹ Type@j }} /\ j <= i) as [j []] by mauto 3.
+    assert {{ ⊢ Γ, A }} by mauto 3.
+    assert (exists j, {{ Γ, A ⊢a B ⟹ Type@j }} /\ j <= i) as [j' []] by mauto 3.
+    assert (max j j' <= i) by lia.
+    econstructor; mauto 3 using alg_subtyping_complete.
+  - assert (exists j, {{ Γ ⊢a A ⟹ Type@j }} /\ j <= i) as [j []] by mauto 3.
+    assert {{ ⊢ Γ, A }} by mauto 3.
+    assert (exists j, {{ Γ, A ⊢a B ⟹ Type@j }} /\ j <= i) as [j' []] by mauto 3.
+    assert {{ Γ ⊢ A : Type@j }}.
+    {
+      eapply alg_type_infer_sound in H3; mauto 3.
+    }
+    assert {{ Γ, A ⊢ B : Type@j' }}. {
+      eapply alg_type_infer_sound in H6; mauto 3.
+    }
+    assert (exists WA, nbe_ty Γ A WA /\ {{ Γ ⊢ A ≈ WA : Type@j }}) as [WA []] by mauto 3 using soundness_ty.
+    assert (exists WB, nbe_ty {{{ Γ , A }}} B WB /\ {{ Γ , A ⊢ B ≈ WB : Type@j' }}) as [WB []] by mauto 3 using soundness_ty.
+    assert {{ Γ ⊢ WA : Type@j }} by (gen_presups; mauto 3).
+    assert {{ Γ , ^(WA :exp) ⊢ WB : Type@j' }}.
+    {
+      gen_presups.
+      eapply @ctxeq_exp with (Γ:={{{Γ,A}}}); mauto 3.
+    }
+    assert {{ Γ ⊢ ^ n{{{ Σ WA WB }}} ⊆ Σ A B }}.
+    { eapply wf_subtyp_sigma with (i:=max j j'); mauto 3
+      using lift_exp_eq_max_left, lift_exp_eq_max_right, lift_exp_max_left, lift_exp_max_right.
+    }
+    assert {{ Γ ⊢a ⟨ M : A; N : B ⟩ ⟹ Σ WA WB }} by (econstructor; mauto 3).
+    mauto 3 using alg_subtyping_complete.
+  - assert {{ Γ ⊢a M ⟸ Σ A B }} by mauto 3.
+    assert (exists A' B', {{ Γ ⊢a M ⟹ Σ A' B' }} /\ {{ Γ ⊢ A' ≈ A : Type@i }} /\ {{ Γ, A ⊢a B' ⊆ B }}) as [A' [B' [? []]]] by mauto 3.
+    assert {{ Γ ⊢a A' ⊆ A }} by mauto 3 using alg_subtyping_complete.
+    mauto 3.
+  - assert {{ Γ ⊢a M ⟸ Σ A B }} by mauto 3.
+    assert (exists A' B', {{ Γ ⊢a M ⟹ Σ A' B' }} /\ {{ Γ ⊢ A' ≈ A : Type@i }} /\ {{ Γ, A ⊢a B' ⊆ B }}) as [A' [B' [? []]]] by mauto 3.
+    assert {{ Γ ⊢ M : Σ A' B' }} by (eapply alg_type_sound in H4; mauto 3).
+    assert (exists j, {{ Γ ⊢ Σ A' B' : Type@j }}) as [j] by (gen_presups; eauto 2).
+    apply wf_sigma_inversion' in HA.
+    apply wf_sigma_inversion' in H8. destruct_all.
+    assert {{ Γ, ^(A:exp) ⊢ B' : Type@j }} by mauto 4.
+    assert {{ Γ, A ⊢ B' ⊆ B }}. {
+      eapply alg_subtyping_sound with (i:=max i0 j); mauto 3 using lift_exp_max_left, lift_exp_max_right.
+    }
+    assert (exists W, nbe_ty Γ {{{ B'[Id,,fst M] }}} W /\ {{ Γ ⊢ B'[Id,,fst M] ≈ W : Type@j }}) as [W []].  {
+      eapply soundness_ty; mauto 3.
+      eapply wf_conv'; [eapply wf_exp_sub |]; mauto 3.
+      econstructor; mauto 3.
+    }
+    assert {{ Γ ⊢ B'[Id,,fst M] ⊆ B[Id,,fst M] }} by (eapply wf_subtyp_subst; mauto 3).
+    assert {{ Γ ⊢ W ⊆ B[Id,,fst M] }} by (transitivity {{{ B'[Id,,fst M] }}}; mauto 3).
+    mauto using alg_subtyping_complete.
+  - assert (exists W, nbe_ty Γ A W /\ {{ Γ ⊢ A ≈ W : Type@i }}) as [W []] by (eapply soundness_ty; mauto 3).
+    econstructor; mauto 4 using alg_subtyping_complete.
+  - assert (exists j, {{ Γ ⊢a A ⟹ Type@j }} /\ j <= i) as [j []] by mauto 3.
+    econstructor; [econstructor |]; mauto 3 using alg_subtyping_complete.
+  - assert (exists j, {{ Γ ⊢a A ⟹ Type@j }} /\ j <= i) as [j []] by mauto 3.
+    assert {{ Γ ⊢a M ⟸ A }} by eauto 2.
+    assert (exists C, nbe_ty Γ A C /\ {{ Γ ⊢ A ≈ C : Type@i }}) as [C []] by mauto 3 using soundness_ty.
+    assert (exists W, nbe Γ M A W /\ {{ Γ ⊢ M ≈ W : A }}) as [W []] by mauto 3 using soundness.
+    econstructor; mauto 3.
+    assert {{ Γ ⊢ ^n{{{ Eq C W W }}} ≈ Eq A M M : Type@i }} by mauto 3.
+    mauto 3 using alg_subtyping_complete.
+  - assert (exists k, {{ Γ ⊢a A ⟹ Type@k }} /\ k <= i) as [k []] by mauto 3.
+    assert (exists l, {{ Γ, A, A[Wk], Eq A[Wk∘Wk] #1 #0 ⊢a B ⟹ Type@l }} /\ l <= j) as [l []] by mauto 3.
+    assert {{ Γ, A ⊢s Wk : Γ }} by mauto 3.
+    assert {{ Γ, A ⊢ A[Wk] : Type@i }} by mauto 3.
+    assert {{ ⊢ Γ, A, A[Wk] }} by mauto 3.
+    assert {{ Γ, A, A[Wk] ⊢ Eq A[Wk∘Wk] #1 #0 : Type@i }} by mauto 3.
+    assert {{ Γ, A, A[Wk], Eq A[Wk∘Wk] #1 #0 ⊢ B : ^n{{{ Type@j }}} }} by mauto 3 using alg_type_infer_sound.
+    assert {{ Γ ⊢s Id,,M1,,M2,,N : Γ, A, A[Wk], Eq A[Wk∘Wk] #1 #0 }} by mauto 2.
+    assert {{ Γ ⊢ B[Id,,M1,,M2,,N] : Type@j }} by mauto 2.
+    assert (exists C, nbe_ty Γ {{{ B[Id,,M1,,M2,,N] }}} C /\ {{ Γ ⊢ B[Id,,M1,,M2,,N] ≈ C : Type@j }}) as [C []] by mauto 3 using soundness_ty.
+    econstructor; [econstructor |]; mauto 4 using alg_subtyping_complete.
+Qed.
+
+#[export]
+Hint Resolve alg_type_check_complete : mcpts.
+
+Corollary alg_type_infer_complete : forall {Γ A M},
+    user_exp M ->
+    {{ Γ ⊢ M : A }} ->
+    exists B, {{ Γ ⊢a M ⟹ B }} /\ {{ Γ ⊢a B ⊆ A }}.
+Proof.
+  intros.
+  assert {{ Γ ⊢a M ⟸ A }} as Hcheck by mauto 4 using alg_type_check_complete.
+  inversion_clear Hcheck.
+  firstorder.
+Qed.
+
+#[export]
+Hint Resolve alg_type_infer_complete : mcpts.
+
+Corollary alg_type_infer_typ_complete : forall {Γ i A},
+    user_exp A ->
+    {{ Γ ⊢ A : Type@i }} ->
+    exists j, {{ Γ ⊢a A ⟹ Type@j }} /\ j <= i.
+Proof.
+  mauto 4 using alg_type_check_complete.
+Qed.
+
+#[export]
+Hint Resolve alg_type_infer_typ_complete : mcpts.
+
+Corollary alg_type_infer_pi_complete : forall {Γ i A},
+    user_exp A ->
+    {{ Γ ⊢ A : Type@i }} ->
+    exists j, {{ Γ ⊢a A ⟹ Type@j }} /\ j <= i.
+Proof.
+  mauto 4 using alg_type_check_complete.
+Qed.
+
+#[export]
+Hint Resolve alg_type_infer_pi_complete : mcpts.
